---
title: "Montgomery Ladder in ECC"
date: "2021-04-21 21:11:18+02:00"
aliases:
  - "../notes/2021/04/montgomery-ladder"
note-tags:
  - "math"
  - "cryptography"
katex: "True"
type: "note"
---

This is a technique to efficiently
calculate the x coordinate $\bold{x}(nP)$
given the x coordinate of a point on a Montgomery curve $\bold{x}(P)$.
This method is also easily implemented in a constant-time way.

This works for curves:

$$
By^2 = x^3 + Ax^2 + x
$$

Satisfying $B(A^2 - 4) \neq 0$.

# In Summary

The ladder itself

```go
func ScalarMul(n Scalar, x Field) Field {
  nP := Projective{1, 0}
  n1P := Projective{x, 1}

  swap := 0
  for b := range n.msb .. n.lsb {
    swap ^= b
    condSwap(swap, nP, n1P)
    swap = b

    nP, n1P = step0(x, nP, n1P)
  }
  condSwap(swap, nP, n1P)
  return nP.X / nP.Z
}
```

Implementing the individual step:

```go
// In field elements of course
const A24 = (A - 2) / 4

func step0(x Field, nP, n1P Projective) (Projective, Projective) {
  double_X := nP.X + nP.Z
  double_Z := nP.X - nP.Z
  // Addition
  add_X := n1P.X + n1P.Z
  add_Z := nP.X - nP.Z
  add_X *= double_Z
  add_Z *= double_X
  tmp := add_X - add_Z
  add_X += add_Z
  add_Z = tmp
  add_X.square()
  add_Z.square()
  add_Z *= x
  // Now we can do doubling
  double_X.square()
  double_Z.square()
  // Store for later
  Xn_plus_Zn_squared := double_X
  double_X *= double_Z
  tmp = Xn_plus_Zn_squared - double_Z
  double_Z = A24 * tmp
  double_Z += Xn_plus_Zn_squared
  double_Z *= tmp
  return (
    Projective{double_X, double_Z},
    Projective{add_X, add_Z}
  )
}
```

This could be optimized to reuse nP and n1P's buffers better as well

# Doubling Formula

Given a point $P = (x, y)$, the formula for $2P$ is given by:

$$
\begin{aligned}
&x_2 = B \lambda^2 - A - 2x \cr
&y_2 = \lambda (x - x_2) - y
\end{aligned}
$$

where:

$$
\lambda = \frac{3x^2 + 2Ax + 1}{2By}
$$

(This formula is derived geometrically. $\lambda$ is the slope of the
tangent line to the curve at the point $P$.)

Because $\lambda^2$ features $By^2$ in the denominator, we can replace
that with $x^3 + Ax^2 + x$, and then calculate out the following
identity:

$$
x_2 = \frac{(x^2 - 1)^2}{4(x^3 + Ax^2 + x)}
$$

This formula calculates $\bold{x}(2P)$ given only $\bold{x}(P)$,
and can be shown to be valid in other edge cases.
See: [^1].

## Projective Form

If we use projective coordinates, then we have $x = X / Z$. Plugging
this into the formula we had above, we get:

$$
x_2 = \frac{(X^2 - Z^2)^2}{4ZX(X + AXZ + Z^2)}
$$

In other terms, this means we have:

$$
\begin{aligned}
&X_2 = (X^2 - Z^2)^2 \cr
&Z_2 = 4XZ(X + AXZ + Z^2)
\end{aligned}
$$

If we calculate this directly, a point doubling takes:

$$
2 \bold{M} + 3 \bold{S} + 2 \bold{C}
$$

We can re-arrange things to allow more sharing:

$$
\begin{aligned}
&X_2 = (X + Z)^2(X - Z)^2 \cr
&Z_2 = ((X + Z)^2 - (X - Z)^2)\left(
  (X + Z)^2 + \frac{A - 2}{4}((X + Z)^2 - (X - Z)^2)
\right)
\end{aligned}
$$

If you note that:

$$
(X + Z)^2 - (X - Z)^2 = 4XZ
$$

The correctness of this formula becomes relatively clear.

This adjusted formula takes:

$$
2 \bold{M} + 2 \bold{S}  + \bold{C}
$$

# Addition Formula

In can be shown that given $P$ and $Q$, we have:

$$
\bold{x}(P + Q)\bold{x}(Q - P) =
\frac{
  (\bold{x}(P)\bold{x}(Q) - 1)^2
}{
  (\bold{x}(Q) - \bold{x}(P))^2
}
$$

(This is a monstrous PITA, see [^1].)

In projective coordinates $[X_P, Z_P],\ [X_Q, Z_Q]$, we get:

$$
\bold{x}(P + Q) \frac{X_{Q - P}}{Z_{Q - P}}
= \frac{(X_P X_Q - Z_P Z_Q)^2}{(X_Q Z_P - X_P Z_Q)^2}
$$

This gives us the following formulas for addition:

$$
\begin{aligned}
&X_{P + Q} = Z_{Q - P}(X_P X_Q - Z_P Z_Q)^2 \cr
&Z_{P + Q} = X_{Q - P}(X_Q Z_P - X_P Z_Q)^2
\end{aligned}
$$

Unlike with doubling, we need to have calculated $P - Q$ prior.
In practice, this constraint is easily accomodated.

This formula requires:

$$
6 \bold{M} + 2 \bold{S}
$$

To simplify it, first note that because of the properties of projective
coordinates, multiplying both $X$ and $Z$ by $4$ gives us the same point:

$$
\begin{aligned}
&X_{P + Q} = 4Z_{Q - P}(X_P X_Q - Z_P Z_Q)^2 \cr
&Z_{P + Q} = 4X_{Q - P}(X_Q Z_P - X_P Z_Q)^2
\end{aligned}
$$

A bit of toil gives us the following formula:

$$
\begin{aligned}
&X_{P + Q} = Z_{Q - P}(
  (X_P - Z_P)(X_Q + Z_Q) + (X_P + Z_P)(X_Q - Z_Q)
)^2 \cr
&Z_{P + Q} = X_{Q - P}(
  (X_P - Z_P)(X_Q + Z_Q) - (X_P + Z_P)(X_Q - Z_Q)
)^2 \cr
\end{aligned}
$$

This gives us an improved:

$$
4 \bold{M} + 2 \bold{S}
$$

In practice, we'll always have $Z_{Q - P}$ as $1$, and $X_{Q - P}$
as a small constant, giving us:

$$
2 \bold{M} + 2 \bold{S} + \bold{C}
$$

# Combined Formula

In practice, you have $(X_2, Z_2)$ and $(X_3, Z_3)$, and calculate
$(X_4, Z_4)$ as well as $(X_5, Z_5)$ together, giving you the following
combined formula:

![](../Images/8c2129bf1257cee49913be91d83c3cf18bd21a41fc50b958735b431a663f54e9.png)

(See: [^1])

# Ladder

One simple way to calculate $kP$ is as follows. Iterate over the bits
of $k$ from most to least significant. If a bit $b = 0$, set:

$$
P \leftarrow 2P
$$

If $b = 1$, then set:

$$
P \leftarrow 2P + P
$$

Our addition formula works well when we have $P_n$ and
$P_{n + 1}$, and want to calculate $P_{2n + 1}$, since the difference
is $P_1 = P$, a point we already know.

At each iteration, as we rise up to $P_k$, our final value, we
want to keep this property, and keep the successive values around.

This, when $b = 0$, we do:

$$
(P_n, P_{n + 1}) \mapsto (P_{2n}, P_{2n + 1})
$$

The first value comes from point doubling $P_n$, and the
second from differential point addition, using the fact
that the difference is $P_1$.

When $b = 1$, we want to do:

$$
(P_n, P_{n + 1}) \mapsto (P_{2n + 1}, P_{2n + 2})
$$

We can calculate the first value through point addition, and the
second through point doubling.

In fact, if we define these two functions as $\text{step}_0$,
and $\text{step}_1$ respectively, we notice that $\text{step}_1$
comes from swapping the input, and then the output.
With:

$$
\text{swap}(P, Q) := (Q, P)
$$

We have:

$$
\text{step}_1 = \text{swap};\text{step}_0;\text{swap}
$$

Thus, an algorithm for doing our ladder would be:

```txt
for b in bits:
  if b == 1:
    swap(P, Q)
  (P, Q) = step0(P, Q)
  if b == 1:
    swap(P, Q)
return P
```

We can make this "constant-time", by replacing our branching
with a conditional swap:

```txt
for b in bits:
  cswap(b, P, Q)
  (P, Q) = step0(P, Q)
  cswap(b, P, Q)
return P
```

If we have two conditional swaps chained together

```txt
cswap(bits[i], P, Q)
cswap(bits[i - 1], P, Q)
```

Which happens between iterations, notice that this is effectively:

```txt
cswap(bits[i] ^ bits[i - 1], P, Q)
```

because of this, we can effectively do:

```txt
cswap(bits[N - 1], P, Q)
step0(P, Q)
cswap(bits[N - 1] ^ bits[N - 1], P, Q)
step0(P, Q)
...
cswap(bits[1] ^ bits[0], P, Q)
step0(P, Q)
cswap(bits[0], P, Q)
```

Noting that `0 ^ bits[N - 1] = bits[N - 1]`, we can effectively do:

```txt
swap := 0
for b in bits:
  swap ^= b
  cswap(swap, P, Q)
  swap = b
  step0(P, Q)
cswap(swap, P, Q)
return P
```

This allows us to efficiently compute whether or not we need to swap.

This is the gist of things, see the summary up top for more useable
pseudo-code.

# References

[^1]

[^1]: [[1] Bernstein, Daniel J., Lange, Tanja - Montgomery Curves and the Montgomery Ladder (2017)](https://eprint.iacr.org/2017/293.pdf)